theories/FOL/DecidableEnumerable.v
@@ -89,7 +89,7 @@ Qed.
 
 Definition cumulative {X} (L: nat -> list X) :=
   forall n, exists A, L (S n) = L n ++ A.
-Hint Extern 0 (cumulative _) => intros ?; cbn; eauto.
+Hint Extern 0 (cumulative _) => intros ?; cbn; eauto : core.
 
 Lemma cum_ge {X} (L: nat -> list X) n m :
   cumulative L -> m >= n -> exists A, L m = L n ++ A.
@@ -148,7 +148,7 @@ Class enumT X :=
   }.
 
 Arguments L_T {_ _} _, _ {_} _.
-Hint Immediate cum_T.
+Hint Immediate cum_T : core.
 
 Lemma discrete_bool : discrete bool.
 Proof.
