theories/ILL/Bsm/bsm_defs.v
@@ -294,7 +294,7 @@ Tactic Notation "bsm" "inv" "POP" "any" "with" hyp(H) constr(a) constr(c) constr
 Tactic Notation "bsm" "inv" "PUSH" "with" hyp(H) constr(a) constr(c) :=
      apply bsm_steps_PUSH_inv with (x := a) (b := c) in H; auto.
 
-Hint Immediate bsm_sss_fun.
+Hint Immediate bsm_sss_fun : core.
 
 (* The Halting problem for BSM *)
   
