theories/Problems/cbvLambda.v
@@ -4,4 +4,4 @@ From Undecidability.L Require Import L.
 
 (* Call-by-Value Lambda Calculus as a Model of Computation in Coq. Yannick Forster and Gert Smolka. Journal of Automated Reasoning (2018). https://www.ps.uni-saarland.de/extras/L-computability/ *)
 
-About eva. (* Halting problem for call-by-value lambda-calculus *)
+Check eva. (* Halting problem for call-by-value lambda-calculus *)
